rename copy_insert to copy_log_sq and writing tweaks

rkt/copy_insert.rkt
@@ -1,15 +1,15 @@
 #lang at-exp s-exp "tmonad.rkt"
 (require "insert.rkt")
-(provide copy_insert)
+(provide copy_log_sq)
 (Fixpoint
- copy_insert #:implicit @A{Set} @x{A} @n{nat}
+ copy_log_sq #:implicit @A{Set} @x{A} @n{nat}
  #:measure n
  #:returns @{bin_tree}
  (match (n)
    [0 => (<== bt_mt)]
    [(S n′) 
     => 
-    (bind ((t (copy_insert x (div2 n′))))
+    (bind ((t (copy_log_sq x (div2 n′))))
           (if (even_odd_dec n′)
               (<== (bt_node x t t))
               (bind ((s (insert x t)))
